CertiGC/verif_forward_roots.v
@@ -1,42 +1,172 @@
 Require Import CertiGraph.CertiGC.gc_spec.
 
+Lemma frames_rep_ptr_or_null: forall sh frames,
+  frames_rep sh frames |-- !! is_pointer_or_null (frames_adr frames).
+  Proof.
+    destruct frames as [|[???]?]; simpl; entailer.
+  Qed.
+
+Hint Resolve frames_rep_ptr_or_null : saturate_local.
+
+Lemma frames_rep_valid_pointer: forall sh frames, 
+   sepalg.nonidentity sh ->
+   frames_rep sh frames |-- valid_pointer (frames_adr frames).
+Proof.
+  intros.
+  destruct frames as [|[???]?]; simpl frames_adr; simpl frames_rep; auto with valid_pointer.
+Qed.
+Hint Resolve frames_rep_valid_pointer: valid_pointer.
+
+Definition ti_rep (sh: share) (t_info: thread_info) p :=
+  data_at sh thread_info_type (Vundef,(Vundef,(ti_heap_p t_info,
+       (ti_args t_info, (ti_fp t_info, (vptrofs (ti_nalloc t_info), nullval)))))) p.
+
 Lemma body_forward_roots: semax_body Vprog Gprog f_forward_roots forward_roots_spec.
 Proof.
-  start_function. unfold fun_info_rep.
-  assert_PROP (isptr fi) by entailer.
-  assert_PROP (isptr ti) by (unfold thread_info_rep; entailer).
-  assert (0 <= 1 < Zlength (live_roots_indices f_info) + 2) by (split; rep_lia).
-  do 3 forward. simpl align. rewrite Znth_pos_cons, Znth_0_cons by lia.
-  simpl sem_binary_operation'.
-  replace (force_val (sem_add_ptr_int (if Archi.ptr64 then tulong else tuint)
-                                      Signed fi (vint 2))) with
-      (offset_val (if Archi.ptr64 then 16 else 8) fi) by
-      (rewrite sem_add_pi'; auto; rep_lia).
-  remember (Zlength (live_roots_indices f_info)) as n.
-  replace_SEP 1 (fun_info_rep rsh f_info fi) by entailer.
-  assert (Zlength roots = Zlength (live_roots_indices f_info)). {
-    destruct H as [_ [? _]]. red in H.
-    rewrite <- (Zlength_map _ _ (flip Znth (ti_args t_info))), <- H, Zlength_map.
-    reflexivity. }
-  forward_for_simple_bound
-    n
-    (EX i: Z, EX g' : LGraph, EX t_info': thread_info, EX roots' : roots_t,
-     PROP (forward_roots_loop from to f_info (nat_inc_list (Z.to_nat i))
-                              roots g roots' g';
+  start_function.
+  unfold thread_info_rep. Intros.
+  assert_PROP (is_pointer_or_null (ti_fp t_info)). {
+    unfold ti_fp.
+    destruct (ti_frames t_info) as [|[???]]; simpl frames_rep; entailer!.
+  }
+  forward.
+  fold (ti_rep sh t_info ti).
+  forward_while (EX frames0: list frame, EX frames: list frame, 
+                 EX g': LGraph, EX t_info': thread_info, EX roots': roots_t,
+      PROP (forward_roots_loop from to (nat_inc_list (length (frames2roots frames0))) roots g roots' g';
+            thread_info_relation t_info t_info';
+            super_compatible (g', t_info', roots') outlier;
+            forward_condition g' t_info' from to)
+      LOCAL (temp _frame (frames_adr frames);
+             temp _from_start (gen_start g' from);
+             temp _from_limit (limit_address g' t_info' from);
+             temp _next (next_address t_info' to))
+      SEP (all_string_constants rsh gv;
+           outlier_rep outlier;
+           graph_rep g';
+           ti_rep sh t_info ti;
+           frames_rep sh frames;
+           frames_rep sh frames -* frames_rep sh (ti_frames t_info');
+         heap_struct_rep sh (map space_tri (spaces (ti_heap t_info')))
+           (ti_heap_p t_info); heap_rest_rep (ti_heap t_info')))%assert.
+  - Exists (@nil frame) (ti_frames t_info) g t_info roots.
+    entailer!.
+    split. apply frl_nil. apply tir_id.    
+    apply wand_sepcon_adjoint; cancel. 
+  - entailer!.
+  - destruct frames as [|[a r s] frames']; [ contradiction HRE; auto | ].
+    simpl frames_rep.
+    Intros.
+    simpl frames_adr.
+    forward.
+    forward. {
+      entailer!. clear - H13. auto with field_compatible.
+      unfold field_address0. rewrite if_true.
+      destruct H13. destruct r; try contradiction. apply I.
+      eapply field_compatible0_cons_Tarray; try eassumption. reflexivity. rep_lia.
+    }
+  forward.
+  forward_loop (EX i: Z, EX g' : LGraph, EX t_info': thread_info, EX roots' : roots_t,
+     PROP (forward_roots_loop from to 
+              (nat_inc_list (length (frames2roots frames0) + Z.to_nat i)) roots g roots' g';
            thread_info_relation t_info t_info';
-           super_compatible (g', t_info', roots') f_info outlier;
+           super_compatible (g', t_info', roots') outlier;
            forward_condition g' t_info' from to)
-     LOCAL (temp _args (offset_val (if Archi.ptr64 then 24 else 12) ti);
-            temp _n (Z2val n);
-            temp _roots (offset_val (if Archi.ptr64 then 16 else 8) fi);
+     LOCAL (temp _frame (frames_adr frames');
+            temp _curr (field_address0 (tarray int_or_ptr_type (Zlength s)) (SUB i) r);
+            temp _limit  (field_address0 (tarray int_or_ptr_type (Zlength s)) (SUB Zlength s) r);
             temp _from_start (gen_start g' from);
             temp _from_limit (limit_address g' t_info' from);
             temp _next (next_address t_info' to))
      SEP (all_string_constants rsh gv;
-          fun_info_rep rsh f_info fi;
           outlier_rep outlier;
           graph_rep g';
-          thread_info_rep sh t_info' ti))%assert.
+          ti_rep sh t_info ti;
+          data_at sh (Tstruct _stack_frame noattr)
+            (field_address0 (tarray int_or_ptr_type (Zlength s)) (SUB Zlength s) r,
+            (r, frames_adr frames')) a;
+          data_at sh (tarray int_or_ptr_type (Zlength s)) s r;
+          frames_rep sh frames';
+          (data_at sh (Tstruct _stack_frame noattr)
+            (field_address0 (tarray int_or_ptr_type (Zlength s)) (SUB Zlength s) r,
+            (r, frames_adr frames')) a
+            * data_at sh (tarray int_or_ptr_type (Zlength s)) s r
+            * frames_rep sh frames') -* frames_rep sh (ti_frames t_info');
+          heap_struct_rep sh (map space_tri (spaces (ti_heap t_info'))) (ti_heap_p t_info);
+          heap_rest_rep (ti_heap t_info')
+     ))%assert.
+   + Exists 0 g' t_info' roots'. entailer!.
+     split. change (Z.to_nat 0) with O. rewrite Nat.add_0_r. auto.
+     rewrite arr_field_address0 by (auto with field_compatible; rep_lia).
+     clear - H15; destruct H15 as [? _]; destruct r; try contradiction; simpl. normalize. 
+   + Intros i g'' t_info'' roots''.
+     forward_if.
+     *  admit.  (* true, but tedious *)
+     * forward_call (rsh, sh, gv, ti, g'', t_info'', roots'', outlier, from,
+         to, 0, (@inl _ (VType*Z) (Zlength (frames2roots frames0) + i))).
+      --  simpl firstn. entailer!. repeat f_equal.
+          admit. (* plausible *)
+      -- unfold thread_info_rep.
+         fold (ti_rep sh t_info'' ti).
+         replace (ti_rep sh t_info'' ti) with (ti_rep sh t_info ti) by admit. (* plausible *)
+         replace (ti_heap_p t_info'') with (ti_heap_p t_info) by admit. (* plausible *)
+         cancel.
+         eapply derives_trans; [apply modus_ponens_wand |].
+         cancel.
+      -- admit. (* whatever *)
+      -- Intros vret.
+         destruct vret as ((g3,t_info3),roots3). simpl fst in *. simpl snd in *.
+         forward.
+         ++ entailer!. admit. (* easy *)
+         ++ Exists (i+1) g3 t_info3 roots3.
+            entailer!.
+            ** admit.  (* some things to prove here *)
+            ** unfold thread_info_rep. fold (ti_rep sh t_info3 ti).
+               replace (ti_rep sh t_info3 ti) with (ti_rep sh t_info ti) by admit. (* plausible *)
+               replace (ti_heap_p t_info3) with (ti_heap_p t_info) by admit. (* plausible *)
+               cancel.
+               set (A := (data_at _ (Tstruct _stack_frame _) _ _ * _ * _)%logic).
+               clear H11 H22 H21 H20 H19 H18 H17.
+               Search (_ |-- _ * (_ -* _)).
+               Search tir
+               red in H16.
+               Print thread_info_relation.
+               admit. (* problematic *)
+
+              
+         set (B := (data_at _ (Tstruct _stack_frame _) _ _ * _ * _)%logic).
+         set (C := frames_rep _ _).
+         sep_apply (modus_ponens_wand B C).
+         
+         (B*C) (frames_rep sh frames'))
+
+         Search spaces thread_info_relation.
+     simpl.
+     unfold forward_p_address, frame_root_address. simpl.
+     unfold weak_valid_pointer.
+     Search weak_valid_pointer.
+     auto 50 with valid_pointer.
+     unfold sameblock.
+     simpl sameblock.
+     auto 50 with valid_pointer.
+     Search denote_tc_test_order.
+     rewrite arr_field_address0 by (auto with field_compatible; rep_lia).
+
+   assert (foo: environ->mpred) by admit.
+
+     forward_if foo.
+        Print heap_rest_rep.
+     
+     cancel.
+     
+     unfold limit_address.
+       rewrite arr_field_address0 by (auto with field_compatible; rep_lia).
+       simpl.
+     unfold field_address0. rewrite if_true. simpl. clear - H15.
+     auto with field_compat
+     destruct H15, r; try contradiction. simpl. reflexivity. auto.
+     clear - H3.
+
   - pose proof lri_range f_info. unfold MAX_UINT in H6. subst n; lia.
   - Exists g t_info roots. destruct H as [? [? [? ?]]]. entailer!.
     split; [|split]; try easy. unfold nat_inc_list. simpl. constructor.
