CertiGC/verif_do_generation.v
@@ -2,6 +2,53 @@ Require Import CertiGraph.CertiGC.gc_spec.
 
 Local Open Scope logic.
 
+Lemma ptrofs_divs_repr
+	 : forall i j : Z,
+       Ptrofs.min_signed <= i <= Ptrofs.max_signed ->
+       Ptrofs.min_signed <= j <= Ptrofs.max_signed ->
+       Ptrofs.divs (Ptrofs.repr i) (Ptrofs.repr j) = 
+       Ptrofs.repr (i ÷ j).
+Proof.
+  intros.
+  unfold Ptrofs.divs.
+  rewrite ?Ptrofs.signed_repr by rep_lia;
+  auto.
+Qed.
+
+Lemma int64_lt_ptrofs_to_int_64:
+  forall x y, Archi.ptr64 = true ->
+    Int64.lt (Ptrofs.to_int64 x) (Ptrofs.to_int64 y) =  Ptrofs.lt x y.
+Proof.
+  intros.
+  unfold Int64.lt, Ptrofs.lt.
+  rewrite <- (Ptrofs.repr_signed x), <- (Ptrofs.repr_signed y).
+  rewrite !ptrofs_to_int64_repr by auto.
+  pose proof Ptrofs.signed_range.
+  unfold Ptrofs.min_signed, Ptrofs.max_signed in H0.
+  unfold Ptrofs.half_modulus, Ptrofs.modulus, Ptrofs.wordsize, 
+    Wordsize_Ptrofs.wordsize in H0. rewrite H in H0.
+  rewrite !Int64.signed_repr by apply H0.
+  rewrite !Ptrofs.signed_repr by apply Ptrofs.signed_range.
+  auto.
+Qed.
+
+Lemma int_lt_ptrofs_to_int_:
+  forall x y, Archi.ptr64 = false ->
+    Int.lt (Ptrofs.to_int x) (Ptrofs.to_int y) =  Ptrofs.lt x y.
+Proof.
+  intros.
+  unfold Int.lt, Ptrofs.lt.
+  rewrite <- (Ptrofs.repr_signed x), <- (Ptrofs.repr_signed y).
+  rewrite !ptrofs_to_int_repr by auto.
+  pose proof Ptrofs.signed_range.
+  unfold Ptrofs.min_signed, Ptrofs.max_signed in H0.
+  unfold Ptrofs.half_modulus, Ptrofs.modulus, Ptrofs.wordsize, 
+    Wordsize_Ptrofs.wordsize in H0. rewrite H in H0.
+  rewrite !Int.signed_repr by apply H0.
+  rewrite !Ptrofs.signed_repr by apply Ptrofs.signed_range.
+  auto.
+Qed.
+
 Lemma body_do_generation: semax_body Vprog Gprog f_do_generation do_generation_spec.
 Proof.
   start_function.
@@ -22,9 +69,10 @@ Proof.
                       (Datatypes.length (g_gen (glabel g))); assumption. }
   assert (Z.of_nat from < MAX_SPACES) by (apply HS; assumption).
   assert (Z.of_nat to < MAX_SPACES) by (apply HS; assumption). clear HS.
-  freeze [0;1;2;3] FR.
+  freeze [0;1;2] FR.
   localize [space_struct_rep sh t_info from; space_struct_rep sh t_info to].
-  unfold space_struct_rep. unfold space_tri. do 5 forward.
+  unfold space_struct_rep. unfold space_tri.
+  forward.
   gather_SEP
     (data_at sh space_type
              _ (space_address t_info from))
@@ -33,63 +81,27 @@ Proof.
   replace_SEP 0 (space_struct_rep sh t_info from * space_struct_rep sh t_info to) by
     (unfold space_struct_rep; entailer!).
   unlocalize [thread_info_rep sh t_info ti].
-  1: apply thread_info_rep_ramif_stable; assumption.
-  remember (space_start (nth_space t_info from)) as from_p.
-  remember (space_start (nth_space t_info to)) as to_p.
-  remember (WORD_SIZE * used_space (nth_space t_info to))%Z as to_used.
-  remember (WORD_SIZE * total_space (nth_space t_info to))%Z as to_total.
-  remember (WORD_SIZE * used_space (nth_space t_info from))%Z as from_used.
-  assert (is_true (sameblock (offset_val from_used from_p) from_p)). {
-    destruct from_p; try contradiction. simpl.
-    destruct peq. 2: contradiction. exact I. }
-  assert (is_true (sameblock (offset_val to_total to_p) (offset_val to_used to_p))). {
-    destruct to_p; try contradiction. simpl.
-    destruct peq. 2: contradiction. exact I. }
-  forward_if True.
-  - forward. entailer!.
-  - destruct from_p; try contradiction. inv_int i. destruct to_p; try contradiction.
-    inv_int i0. simpl in H18; unfold sem_sub_pp in H18;
-                  destruct eq_block in H18; [|easy]. exfalso.
-    rewrite !ptrofs_add_repr, !ptrofs_sub_repr, !if_true in H18 by reflexivity.
-    simpl in H18. replace (ofs0 + to_total - (ofs0 + to_used)) with
-                      (to_total - to_used) in H18 by lia.
-    replace (ofs + from_used - ofs) with from_used in H18 by lia.
-    assert (Ptrofs.min_signed <= from_used <= Ptrofs.max_signed) by
-        (subst; apply used_space_signed_range).
-    assert (Ptrofs.min_signed <= to_total - to_used <= Ptrofs.max_signed) by
-        (subst; apply rest_space_signed_range). unfold Ptrofs.divs in H18.
-    rewrite !Ptrofs.signed_repr in H18 by rep_lia. subst. unfold WORD_SIZE in H18.
-    rewrite <- Z.mul_sub_distr_l, Z.mul_comm, Z.quot_mul,
-    Z.mul_comm, Z.quot_mul in H18 by lia.
-    first [rewrite !ptrofs_to_int_repr in H18 |
-           rewrite !ptrofs_to_int64_repr in H18 by auto]. red in H18.
-    remember (if Archi.ptr64
-              then Int64.lt
-                     (Int64.repr
-                        (total_space (nth_space t_info to) -
-                         used_space (nth_space t_info to)))
-                     (Int64.repr (used_space (nth_space t_info from)))
-              else Int.lt
-                     (Int.repr
-                        (total_space (nth_space t_info to) -
-                         used_space (nth_space t_info to)))
-                     (Int.repr (used_space (nth_space t_info from)))) as lte.
-    simpl in Heqlte. rewrite <- Heqlte in H18. destruct lte; simpl in H18.
-    2: inversion H18. symmetry in Heqlte.
-    match goal with
-    | H : Int64.lt _ _ = true |- _ => apply lt64_repr in H
-    | H : Int.lt _ _ = true |- _ => apply lt_repr in H
-    end.
-    2: apply rest_space_repable_signed.
-    2: apply used_space_repable_signed. clear -H8 H3 Heqlte. red in H3.
-    unfold graph_gen_size, rest_gen_size in H3. rewrite H8 in H3. lia.
-  - Intros. localize [space_struct_rep sh t_info from].
-    unfold space_struct_rep, space_tri. do 2 (forward; [subst from_p; entailer!|]).
+  1: apply thread_info_rep_ramif_stable;  assumption.
+  assert_PROP (isptr (space_address t_info to)). {
+    unfold thread_info_rep. unfold heap_struct_rep.
+    unfold space_address. Intros.
+    entailer!.
+  }
+  forward_call. clear H16. 
+    localize [space_struct_rep sh t_info from].
+    unfold space_struct_rep, space_tri. 
+    forward.
+    forward.
     replace_SEP 0 (space_struct_rep sh t_info from) by
         (unfold space_struct_rep, space_tri; entailer!).
     unlocalize [thread_info_rep sh t_info ti].
     1: apply thread_info_rep_ramif_stable_1; assumption. apply dgc_imply_fc in H0.
-    destruct H0 as [? [? [? ?]]]. rewrite <- Heqfrom_p.
+    remember (space_start (nth_space t_info from)) as from_p.
+    remember (space_start (nth_space t_info to)) as to_p.
+    remember (WORD_SIZE * used_space (nth_space t_info to))%Z as to_used.
+    remember (WORD_SIZE * total_space (nth_space t_info to))%Z as to_total.
+    remember (WORD_SIZE * used_space (nth_space t_info from))%Z as from_used.
+    destruct H0 as [? [? ?]]. 
     replace from_p with (gen_start g from) by
         (subst; unfold gen_start; rewrite if_true; assumption).
     replace (offset_val (WORD_SIZE * total_space (nth_space t_info from))
@@ -105,31 +117,32 @@ Proof.
       - simpl. rewrite offset_offset_val. f_equal.
       - destruct H as [[_ [_ ?]] _]. unfold field_compatible in *.
         simpl in *. unfold in_members. simpl. intuition. } thaw FR.
-    forward_call (rsh, sh, gv, fi, ti, g, t_info, f_info, roots, outlier, from, to).
+    forward_call (rsh, sh, gv, ti, g, t_info, roots, outlier, from, to).
     1: intuition. Intros vret. destruct vret as [[g1 t_info1] roots1]. simpl fst in *.
-    simpl snd in *. freeze [0;1;2;3] FR. 
+    simpl snd in *. freeze [0;1;2] FR.  
     replace (space_address t_info from) with (space_address t_info1 from) by
-        (unfold space_address; rewrite (proj1 H26); reflexivity).
+        (unfold space_address; rewrite (proj1 H23); reflexivity).
     assert (space_start (nth_space t_info1 from) = gen_start g1 from). {
-      destruct H23 as [? _]. destruct H25 as [_ [? _]].
-      destruct (gt_gs_compatible _ _ H23 _ H25) as [? _]. rewrite <- H27.
+      destruct H20 as [? _]. destruct H22 as [_ [? _]].
+      destruct (gt_gs_compatible _ _ H20 _ H22) as [? _]. rewrite <- H24.
       unfold gen_start. rewrite if_true by assumption. reflexivity. }
     assert (isptr (space_start (nth_space t_info1 from))). {
-      rewrite H27. unfold gen_start. destruct H25 as [_ [? _]].
+      rewrite H24. unfold gen_start. destruct H22 as [_ [? _]].
       rewrite if_true by assumption. apply start_isptr. }
     localize [space_struct_rep sh t_info1 from].
-    unfold space_struct_rep, space_tri. do 2 forward.
+    unfold space_struct_rep, space_tri. 
+    do 2 forward.
     replace_SEP 0 (space_struct_rep sh t_info1 from) by
         (unfold space_struct_rep, space_tri; entailer!).
     unlocalize [thread_info_rep sh t_info1 ti].
-    1: apply thread_info_rep_ramif_stable_1; assumption. thaw FR. rewrite H27.
+    1: apply thread_info_rep_ramif_stable_1; assumption. thaw FR. rewrite H24.
     replace (offset_val (WORD_SIZE * total_space (nth_space t_info1 from))
                         (gen_start g1 from)) with (limit_address g1 t_info1 from) by
         (unfold limit_address, gen_size; reflexivity).
     assert_PROP (offset_val WORD_SIZE (space_address t_info to) =
                  next_address t_info1 to). {
       unfold thread_info_rep. unfold heap_struct_rep. entailer!.
-      unfold space_address, next_address, field_address. rewrite (proj1 H26), if_true.
+      unfold space_address, next_address, field_address. rewrite (proj1 H23), if_true.
       - simpl. rewrite offset_offset_val. f_equal.
       - unfold field_compatible in *. simpl.
         unfold in_members. simpl. intuition. }
@@ -138,66 +151,88 @@ Proof.
     replace (offset_val to_used to_p) with
         (offset_val (- WORD_SIZE)
                     (vertex_address g1 (to, number_of_vertices (nth_gen g to)))) by
-        (rewrite <- (frr_vertex_address _ _ _ _ _ _ _ H5 H24 _ H30); subst;
+        (rewrite <- (frr_vertex_address _ _ _ _ _ _ H5 H21 _ H27); subst;
          unfold vertex_address, vertex_offset, gen_start; simpl;
          rewrite offset_offset_val, H11, H9, if_true by assumption;
-         f_equal; unfold WORD_SIZE; lia). eapply frr_closure_has_v in H30; eauto.
-    destruct H30. simpl in H30, H31.
-    assert (0 < gen_size t_info1 to) by (rewrite <- (proj1 (proj2 H26)); assumption).
-    assert (gen_unmarked g1 to) by (eapply (frr_gen_unmarked _ _ _ _ g _ g1); eauto).
-    forward_call (rsh, sh, gv, fi, ti, g1, t_info1, f_info, roots1, outlier,
-                  from, to, number_of_vertices (nth_gen g to)). 1: intuition.
+         f_equal; unfold WORD_SIZE; lia). eapply frr_closure_has_v in H27; eauto.
+    destruct H27. simpl in H27, H28.
+    assert (0 < gen_size t_info1 to) by (rewrite <- (proj1 (proj2 H23)); assumption).
+    assert (gen_unmarked g1 to) by (eapply (frr_gen_unmarked _ _ _ g _ g1); eauto).
+    forward_call (rsh, sh, gv, ti, g1, t_info1, roots1, outlier,
+                  from, to, number_of_vertices (nth_gen g to)).
     Intros vret. destruct vret as [g2 t_info2]. simpl fst in *. simpl snd in *.
-    forward_if True; Intros; [contradiction | forward; entailer! |].
     replace (space_address t_info1 from) with (space_address t_info2 from) in * by
-        (unfold space_address; rewrite (proj1 H37); reflexivity).
+        (unfold space_address; rewrite (proj1 H34); reflexivity).
     assert (space_start (nth_space t_info2 from) = gen_start g2 from). {
-      destruct H34 as [? _]. destruct H35 as [_ [? _]].
-      destruct (gt_gs_compatible _ _ H34 _ H35) as [? _]. rewrite <- H38.
+      destruct H31 as [? _]. destruct H32 as [_ [? _]].
+      destruct (gt_gs_compatible _ _ H31 _ H32) as [? _]. rewrite <- H35.
       unfold gen_start. rewrite if_true by assumption. reflexivity. }
     assert (isptr (space_start (nth_space t_info2 from))). {
-      rewrite H38. unfold gen_start. destruct H35 as [_ [? _]].
+      rewrite H35. unfold gen_start. destruct H32 as [_ [? _]].
       rewrite if_true by assumption. apply start_isptr. } 
-    freeze [0;1;2;3] FR. localize [space_struct_rep sh t_info2 from].
-    unfold space_struct_rep, space_tri. forward.
+    freeze [0;1;2] FR. localize [space_struct_rep sh t_info2 from].
+    unfold space_struct_rep, space_tri.
+    forward.
     replace_SEP 0 (space_struct_rep sh t_info2 from) by
         (unfold space_struct_rep, space_tri; entailer!).
     unlocalize [thread_info_rep sh t_info2 ti].
     1: apply thread_info_rep_ramif_stable_1; assumption. thaw FR.
-    unfold thread_info_rep. Intros. freeze [0;2;3;4;6] FR. rewrite heap_struct_rep_eq.
+    unfold thread_info_rep. Intros. freeze [0;1;3;4;6] FR. rewrite heap_struct_rep_eq.
     assert_PROP (space_address t_info2 from =
-                 field_address (tarray space_type 12) [ArraySubsc (Z.of_nat from)]
+                 field_address (tarray space_type MAX_SPACES) [ArraySubsc (Z.of_nat from)]
                                (ti_heap_p t_info2)). {
       entailer!. unfold space_address. unfold field_address. rewrite if_true.
       - simpl. f_equal.
       - unfold field_compatible in *. simpl in *. intuition. }
-    rewrite H40. clear H40. Opaque Znth. forward. Transparent Znth. 1: entailer!.
+    rewrite H37. clear H37. Opaque Znth. forward. Transparent Znth.
     rewrite Znth_map by (rewrite spaces_size; rep_lia).
-    rewrite <- nth_space_Znth. unfold space_tri at 2 3. thaw FR.
-    assert (graph_has_gen g2 from) by (destruct H35 as [_ [? _]]; assumption).
+    rewrite <- nth_space_Znth. unfold space_tri at 2 3.
+    simpl fst. simpl snd.
+    assert (FROM_MAX: 0 <= Z.of_nat from < Zlength (map space_tri (spaces (ti_heap t_info2)))). {
+        rewrite Zlength_map.
+        destruct H20 as [[_ [_ ?]] _]; destruct H31 as [[_ [_ ?]] _].
+        apply frr_graph_has_gen with (gen:=from) in H21; auto.
+        rewrite H21 in H4.
+        destruct H33 as [n [? _]].
+        apply svwl_graph_has_gen with (gen:=from) in H33; auto.
+        rewrite H33 in H4.
+        clear - H31 H4.
+        red in H4. split. lia. rewrite Zlength_correct.
+        lia. 
+    }
+    Opaque fst. Opaque snd.
+    forward; rewrite upd_Znth_same by assumption. entailer!.
+    forward; rewrite upd_Znth_same by assumption.
+    rewrite !upd_Znth_twice by assumption.
+    Transparent fst. Transparent snd.
+    thaw FR.
+    assert (graph_has_gen g2 from) by (destruct H32 as [_ [? _]]; assumption).
     rewrite (graph_rep_reset g2 from) by assumption. Intros.     
-    sep_apply (heap_rest_rep_reset g2 t_info2 from (proj1 H34) H40).
-    rewrite <- heap_struct_rep_eq.
-    gather_SEP (data_at _ _ _ _) (heap_struct_rep _ _ _) (heap_rest_rep _).
+    sep_apply (heap_rest_rep_reset g2 t_info2 from (proj1 H31) H37).
+        rewrite <- heap_struct_rep_eq.
+    gather_SEP (data_at _ _ _ _) (frames_rep _ _) (heap_struct_rep _ _ _) (heap_rest_rep _).
     replace_SEP 0 (thread_info_rep sh (reset_nth_heap_thread_info from t_info2) ti).
     + unfold thread_info_rep. simpl ti_heap_p. simpl ti_args. entailer!.
       assert (from < length (spaces (ti_heap t_info2)))%nat by
-          (destruct H34 as [[_ [_ ?]] _]; red in H40; lia). simpl.
-      rewrite (reset_nth_space_Znth _ _ H53), <- nth_space_Znth, <- upd_Znth_map.
+          (destruct H31 as [[_ [_ ?]] _]; red in H37; lia). simpl.
+      rewrite (reset_nth_space_Znth _ _ H49), <- nth_space_Znth, <- upd_Znth_map.
       unfold space_tri at 3. simpl. replace (WORD_SIZE * 0)%Z with 0 by lia.
       rewrite isptr_offset_val_zero by assumption. cancel.
-    + apply super_compatible_reset with (gen := from) in H34.
-      2: { apply (frr_not_pointing from to f_info roots g roots1 g1); auto.
+    + apply super_compatible_reset with (gen := from) in H31.
+      2: { apply (frr_not_pointing from to roots g roots1 g1); auto.
            - clear -H0. destruct H0 as [_ [_ [_ [? _]]]]. assumption.
-           - clear -H. destruct H as [_ [_ [[_ ?] _]]]. assumption. }
+           - clear -H. destruct H as [_ [_ [[_ ?] _]]]. assumption.
+           - apply frl_roots_Zlength in H21; auto. 
+      }
       remember (reset_nth_heap_thread_info from t_info2) as t_info3.
       remember (reset_graph from g2) as g3.
-      assert (do_generation_relation from to f_info roots roots1 g g3) by
+      assert (do_generation_relation from to roots roots1 g g3) by
           (exists g1, g2; split; [|split]; assumption).
       assert (thread_info_relation t_info t_info3). {
         apply tir_trans with t_info2.
         - apply tir_trans with t_info1; assumption.
-        - subst t_info3. apply tir_reset. }
+        - subst t_info3. apply tir_reset. }      
       Exists g3 t_info3 roots1.
-      destruct H34 as [? [? [? ?]]]. entailer!. easy.
+      destruct H32 as [? [? [? ?]]]. entailer!.
 Qed.
+
